src/X509.BasicFields.Extension.fst
@@ -10,16 +10,16 @@ open X509.Base
 
 module B32 = FStar.Bytes
 
-inline_for_extraction
-type x509_extension_t
-  (#k: parser_kind)
-  (#t: Type0)
-  (#p: parser k t)
-  (oid: datatype_of_asn1_type OID)
-  (s: serializer p)
-= { x509_extID      : x:datatype_of_asn1_type OID {x == oid};
-    x509_extCritical: datatype_of_asn1_type BOOLEAN;
-    x509_extValue   : OCTET_STRING `inbound_envelop_tag_with_value_of` s }
+// inline_for_extraction
+// type x509_extension_t
+//   (#k: parser_kind)
+//   (#t: Type0)
+//   (#p: parser k t)
+//   (oid: datatype_of_asn1_type OID)
+//   (s: serializer p)
+// = { x509_extID      : x:datatype_of_asn1_type OID {x == oid};
+//     x509_extCritical: datatype_of_asn1_type BOOLEAN;
+//     x509_extValue   : OCTET_STRING `inbound_envelop_tag_with_value_of` s }
 
 /// tuple repr
 let x509_extension_t'
@@ -34,27 +34,27 @@ let x509_extension_t'
   `tuple2`
  (OCTET_STRING `inbound_envelop_tag_with_value_of` s)
 
-let synth_x509_extension_t
-  (#k: parser_kind)
-  (#t: Type0)
-  (#p: parser k t)
-  (oid: datatype_of_asn1_type OID)
-  (s: serializer p)
-  (x': x509_extension_t' oid s)
-: GTot (x509_extension_t oid s)
-= { x509_extID       = fst (fst x');
-    x509_extCritical = snd (fst x');
-    x509_extValue    = snd x' }
+// let synth_x509_extension_t
+//   (#k: parser_kind)
+//   (#t: Type0)
+//   (#p: parser k t)
+//   (oid: datatype_of_asn1_type OID)
+//   (s: serializer p)
+//   (x': x509_extension_t' oid s)
+// : GTot (x509_extension_t oid s)
+// = { x509_extID       = fst (fst x');
+//     x509_extCritical = snd (fst x');
+//     x509_extValue    = snd x' }
 
-let synth_x509_extension_t'
-  (#k: parser_kind)
-  (#t: Type0)
-  (#p: parser k t)
-  (oid: datatype_of_asn1_type OID)
-  (s: serializer p)
-  (x: x509_extension_t oid s)
-: GTot (x': x509_extension_t' oid s { x == synth_x509_extension_t oid s x' })
-= (x.x509_extID, x.x509_extCritical), x.x509_extValue
+// let synth_x509_extension_t'
+//   (#k: parser_kind)
+//   (#t: Type0)
+//   (#p: parser k t)
+//   (oid: datatype_of_asn1_type OID)
+//   (s: serializer p)
+//   (x: x509_extension_t oid s)
+// : GTot (x': x509_extension_t' oid s { x == synth_x509_extension_t oid s x' })
+// = (x.x509_extID, x.x509_extCritical), x.x509_extValue
 
 let parse_x509_extension_kind
 = parse_asn1_TLV_kind_of_type OID
@@ -69,8 +69,12 @@ let parse_x509_extension
   (#p: parser k t)
   (oid: datatype_of_asn1_type OID)
   (s: serializer p)
-: parser parse_x509_extension_kind (x509_extension_t oid s)
-= parse_asn1_oid_TLV_of oid
+  (#instance_t: Type0)
+  (f: x509_extension_t' oid s -> GTot instance_t)
+  (prf: unit{synth_injective f})
+: parser parse_x509_extension_kind (instance_t)
+=
+  parse_asn1_oid_TLV_of oid
   `nondep_then`
   parse_asn1_TLV_of_type BOOLEAN
   `nondep_then`
@@ -78,7 +82,7 @@ let parse_x509_extension
   `parse_asn1_envelop_tag_with_TLV`
   s)
   `parse_synth`
-  synth_x509_extension_t oid s
+  (prf; f)
 
 let serialize_x509_extension
   (#k: parser_kind)
@@ -86,8 +90,14 @@ let serialize_x509_extension
   (#p: parser k t)
   (oid: datatype_of_asn1_type OID)
   (s: serializer p)
-: serializer (parse_x509_extension oid s)
-= serialize_synth
+  (#instance_t: Type0)
+  (f: x509_extension_t' oid s -> GTot instance_t)
+  (g: instance_t -> x509_extension_t' oid s)
+  (prf: unit{ synth_inverse f g /\
+              synth_injective f })
+: serializer (parse_x509_extension oid s f prf)
+=
+  serialize_synth
   (* p1 *) (parse_asn1_oid_TLV_of oid
             `nondep_then`
             parse_asn1_TLV_of_type BOOLEAN
@@ -95,7 +105,7 @@ let serialize_x509_extension
            (OCTET_STRING
             `parse_asn1_envelop_tag_with_TLV`
             s))
-  (* f2 *) (synth_x509_extension_t oid s)
+  (* f2 *) (f)
   (* s1 *) (serialize_asn1_oid_TLV_of oid
             `serialize_nondep_then`
             serialize_asn1_TLV_of_type BOOLEAN
@@ -103,8 +113,8 @@ let serialize_x509_extension
            (OCTET_STRING
             `serialize_asn1_envelop_tag_with_TLV`
             s))
-  (* g1 *) (synth_x509_extension_t' oid s)
-  (* prf*) ()
+  (* g1 *) (g)
+  (* prf*) (prf)
 
 let lemma_serialize_x509_extension_unfold
   (#k: parser_kind)
@@ -112,19 +122,24 @@ let lemma_serialize_x509_extension_unfold
   (#p: parser k t)
   (oid: datatype_of_asn1_type OID)
   (s: serializer p)
-  (x: x509_extension_t oid s)
+  (#instance_t: Type0)
+  (f: x509_extension_t' oid s -> GTot instance_t)
+  (g: instance_t -> x509_extension_t' oid s)
+  (prf: unit{ synth_inverse f g /\
+              synth_injective f })
+  (x: instance_t)
 : Lemma (
-  serialize (serialize_x509_extension oid s) x ==
-  serialize (serialize_asn1_oid_TLV_of oid) x.x509_extID
+  serialize (serialize_x509_extension oid s f g prf) x ==
+  serialize (serialize_asn1_oid_TLV_of oid) (fst (fst (g x)))
   `Seq.append`
-  serialize (serialize_asn1_TLV_of_type BOOLEAN) x.x509_extCritical
+  serialize (serialize_asn1_TLV_of_type BOOLEAN) (snd (fst (g x)))
   `Seq.append`
-  serialize (OCTET_STRING `serialize_asn1_envelop_tag_with_TLV` s) x.x509_extValue
+  serialize (OCTET_STRING `serialize_asn1_envelop_tag_with_TLV` s) (snd (g x))
 )
 = serialize_nondep_then_eq
   (* s1 *) (serialize_asn1_oid_TLV_of oid)
   (* s2 *) (serialize_asn1_TLV_of_type BOOLEAN)
-  (* in *) (fst (synth_x509_extension_t' oid s x));
+  (* in *) (fst (g x));
   serialize_nondep_then_eq
   (* s1 *) (serialize_asn1_oid_TLV_of oid
             `serialize_nondep_then`
@@ -132,7 +147,7 @@ let lemma_serialize_x509_extension_unfold
   (* s2 *) (OCTET_STRING
             `serialize_asn1_envelop_tag_with_TLV`
             s)
-  (* in *) (synth_x509_extension_t' oid s x);
+  (* in *) (g x);
   serialize_synth_eq
   (* p1 *) (parse_asn1_oid_TLV_of oid
             `nondep_then`
@@ -141,7 +156,7 @@ let lemma_serialize_x509_extension_unfold
            (OCTET_STRING
             `parse_asn1_envelop_tag_with_TLV`
             s))
-  (* f2 *) (synth_x509_extension_t oid s)
+  (* f2 *) (f)
   (* s1 *) (serialize_asn1_oid_TLV_of oid
             `serialize_nondep_then`
             serialize_asn1_TLV_of_type BOOLEAN
@@ -149,8 +164,8 @@ let lemma_serialize_x509_extension_unfold
            (OCTET_STRING
             `serialize_asn1_envelop_tag_with_TLV`
             s))
-  (* g1 *) (synth_x509_extension_t' oid s)
-  (* prf*) ()
+  (* g1 *) (g)
+  (* prf*) (prf)
   (* in *) x
 
 #push-options "--z3rlimit 32 --fuel 4 --ifuel 4"
@@ -160,21 +175,26 @@ let lemma_serialize_x509_extension_size
   (#p: parser k t)
   (oid: datatype_of_asn1_type OID)
   (s: serializer p)
-  (x: x509_extension_t oid s)
+  (#instance_t: Type0)
+  (f: x509_extension_t' oid s -> GTot instance_t)
+  (g: instance_t -> x509_extension_t' oid s)
+  (prf: unit{ synth_inverse f g /\
+              synth_injective f })
+  (x: instance_t)
 : Lemma (
-  Seq.length (serialize (serialize_x509_extension oid s) x) ==
-  length_of_asn1_primitive_TLV x.x509_extID +
-  length_of_asn1_primitive_TLV x.x509_extCritical +
-  length_of_TLV OCTET_STRING (length_of_opaque_serialization s x.x509_extValue) /\
-  length_of_asn1_primitive_TLV x.x509_extCritical == 3
+  Seq.length (serialize (serialize_x509_extension oid s f g prf) x) ==
+  length_of_asn1_primitive_TLV (fst (fst (g x))) +
+  length_of_asn1_primitive_TLV (snd (fst (g x))) +
+  length_of_TLV OCTET_STRING (length_of_opaque_serialization s (snd (g x))) /\
+  length_of_asn1_primitive_TLV (snd (fst (g x))) == 3
 )
-= lemma_serialize_x509_extension_unfold oid s x;
-  lemma_serialize_asn1_oid_TLV_of_size oid x.x509_extID;
+= lemma_serialize_x509_extension_unfold oid s f g prf x;
+  lemma_serialize_asn1_oid_TLV_of_size oid (fst (fst (g x)));
   lemma_serialize_asn1_envelop_tag_with_TLV_size
     OCTET_STRING
     s
-    x.x509_extValue;
-  lemma_serialize_asn1_boolean_TLV_size x.x509_extCritical
+    (snd (g x));
+  lemma_serialize_asn1_boolean_TLV_size (snd (fst (g x)))
 #pop-options
 
 unfold
@@ -184,8 +204,13 @@ let x509_extension_t_inbound
   (#p: parser k t)
   (oid: datatype_of_asn1_type OID)
   (s: serializer p)
+  (#instance_t: Type0)
+  (f: x509_extension_t' oid s -> GTot instance_t)
+  (g: instance_t -> x509_extension_t' oid s)
+  (prf: unit{ synth_inverse f g /\
+              synth_injective f })
 = inbound_sequence_value_of
-  (* s *) (serialize_x509_extension oid s)
+  (* s *) (serialize_x509_extension oid s f g prf)
 
 /// SEQUENCE TLV
 
@@ -199,9 +224,14 @@ let parse_x509_extension_sequence_TLV
   (#p: parser k t)
   (oid: datatype_of_asn1_type OID)
   (s: serializer p)
-: parser parse_x509_extension_sequence_TLV_kind (x509_extension_t_inbound oid s)
+  (#instance_t: Type0)
+  (f: x509_extension_t' oid s -> GTot instance_t)
+  (g: instance_t -> x509_extension_t' oid s)
+  (prf: unit{ synth_inverse f g /\
+              synth_injective f })
+: parser parse_x509_extension_sequence_TLV_kind (x509_extension_t_inbound oid s f g prf)
 = parse_asn1_sequence_TLV
-  (* s *) (serialize_x509_extension oid s)
+  (* s *) (serialize_x509_extension oid s f g prf)
 
 unfold
 let serialize_x509_extension_sequence_TLV
@@ -210,9 +240,14 @@ let serialize_x509_extension_sequence_TLV
   (#p: parser k t)
   (oid: datatype_of_asn1_type OID)
   (s: serializer p)
-: serializer (parse_x509_extension_sequence_TLV oid s)
+  (#instance_t: Type0)
+  (f: x509_extension_t' oid s -> GTot instance_t)
+  (g: instance_t -> x509_extension_t' oid s)
+  (prf: unit{ synth_inverse f g /\
+              synth_injective f })
+: serializer (parse_x509_extension_sequence_TLV oid s f g prf)
 = serialize_asn1_sequence_TLV
-  (* s *) (serialize_x509_extension oid s)
+  (* s *) (serialize_x509_extension oid s f g prf)
 
 unfold
 let lemma_serialize_x509_extension_sequence_TLV_unfold
@@ -221,10 +256,15 @@ let lemma_serialize_x509_extension_sequence_TLV_unfold
   (#p: parser k t)
   (oid: datatype_of_asn1_type OID)
   (s: serializer p)
-  (x: x509_extension_t_inbound oid s)
-: Lemma ( predicate_serialize_asn1_sequence_TLV_unfold (serialize_x509_extension oid s) x )
+  (#instance_t: Type0)
+  (f: x509_extension_t' oid s -> GTot instance_t)
+  (g: instance_t -> x509_extension_t' oid s)
+  (prf: unit{ synth_inverse f g /\
+              synth_injective f })
+  (x: x509_extension_t_inbound oid s f g prf)
+: Lemma ( predicate_serialize_asn1_sequence_TLV_unfold (serialize_x509_extension oid s f g prf) x )
 = lemma_serialize_asn1_sequence_TLV_unfold
-  (* s *) (serialize_x509_extension oid s)
+  (* s *) (serialize_x509_extension oid s f g prf)
   x
 
 unfold
@@ -234,25 +274,29 @@ let lemma_serialize_x509_extension_sequence_TLV_size
   (#p: parser k t)
   (oid: datatype_of_asn1_type OID)
   (s: serializer p)
-  (x: x509_extension_t_inbound oid s)
-: Lemma ( predicate_serialize_asn1_sequence_TLV_size (serialize_x509_extension oid s) x )
+  (#instance_t: Type0)
+  (f: x509_extension_t' oid s -> GTot instance_t)
+  (g: instance_t -> x509_extension_t' oid s)
+  (prf: unit{ synth_inverse f g /\
+              synth_injective f })
+  (x: x509_extension_t_inbound oid s f g prf)
+: Lemma ( predicate_serialize_asn1_sequence_TLV_size (serialize_x509_extension oid s f g prf) x )
 = lemma_serialize_asn1_sequence_TLV_size
-  (* s *) (serialize_x509_extension oid s)
+  (* s *) (serialize_x509_extension oid s f g prf)
   x
 
 open ASN1.Low
 
-inline_for_extraction noextract
-let synth_x509_extension_t'_impl
-  (#k: parser_kind)
-  (#t: Type0)
-  (#p: parser k t)
-  (oid: datatype_of_asn1_type OID)
-  (s: serializer p)
-  (x: x509_extension_t oid s)
-: Tot (x': x509_extension_t' oid s { x' == synth_x509_extension_t' oid s x })
-= (x.x509_extID, x.x509_extCritical), x.x509_extValue
-
+// inline_for_extraction noextract
+// let synth_x509_extension_t'_impl
+//   (#k: parser_kind)
+//   (#t: Type0)
+//   (#p: parser k t)
+//   (oid: datatype_of_asn1_type OID)
+//   (s: serializer p)
+//   (x: x509_extension_t oid s)
+// : Tot (x': x509_extension_t' oid s { x' == synth_x509_extension_t' oid s x })
+// = (x.x509_extID, x.x509_extCritical), x.x509_extValue
 
 //AR: 06/11: this and the next one seem helpers to me?
 inline_for_extraction noextract
@@ -263,7 +307,13 @@ let serialize32_x509_extension_backwards
   (#s: serializer p)
   (oid: datatype_of_asn1_type OID)
   (s32: serializer32_backwards s)
-: serializer32_backwards (serialize_x509_extension oid s)
+  (#instance_t: Type0)
+  (f: x509_extension_t' oid s -> GTot instance_t)
+  (g: instance_t -> x509_extension_t' oid s)
+  (g': (x2: instance_t) -> Tot (x1: x509_extension_t' oid s { x1 == g x2 }))
+  (prf: unit{ synth_inverse f g /\
+              synth_injective f })
+: serializer32_backwards (serialize_x509_extension oid s f g prf)
 = serialize32_synth_backwards
   (* s32*) (serialize32_asn1_oid_TLV_of_backwards oid
             `serialize32_nondep_then_backwards`
@@ -272,10 +322,10 @@ let serialize32_x509_extension_backwards
            (OCTET_STRING
             `serialize32_asn1_envelop_tag_with_TLV_backwards`
             s32))
-  (* f2 *) (synth_x509_extension_t oid s)
-  (* g1 *) (synth_x509_extension_t' oid s)
-  (* g1'*) (synth_x509_extension_t'_impl oid s)
-  (* prf*) ()
+  (* f2 *) (f)
+  (* g1 *) (g)
+  (* g1'*) (g')
+  (* prf*) (prf)
 
 inline_for_extraction noextract
 let serialize32_x509_extension_sequence_TLV_backwards
@@ -285,8 +335,12 @@ let serialize32_x509_extension_sequence_TLV_backwards
   (#s: serializer p)
   (oid: datatype_of_asn1_type OID)
   (s32: serializer32_backwards s)
-: serializer32_backwards (serialize_x509_extension_sequence_TLV oid s)
+  (#instance_t: Type0)
+  (f: x509_extension_t' oid s -> GTot instance_t)
+  (g: instance_t -> x509_extension_t' oid s)
+  (g': (x2: instance_t) -> Tot (x1: x509_extension_t' oid s { x1 == g x2 }))
+  (prf: unit{ synth_inverse f g /\
+              synth_injective f })
+: serializer32_backwards (serialize_x509_extension_sequence_TLV oid s f g prf)
 = serialize32_asn1_sequence_TLV_backwards
-  (* s32 *) (serialize32_x509_extension_backwards oid s32)
-
-let _ = assert (length_of_oid OID_EC_GRP_SECP256R1 == 6)
+  (* s32 *) (serialize32_x509_extension_backwards oid s32 f g g' prf)
