src/RIoT.X509.Extension.fst
@@ -4,77 +4,132 @@ open ASN1.Spec
 open X509.BasicFields.Extension
 open RIoT.X509.CompositeDeviceID
 
-// #set-options "--z3rlimit 8"
-let _ = assert (length_of_oid OID_EC_GRP_SECP256R1 == 6)
-let _ = assert (length_of_asn1_primitive_TLV (Mkbit_string_t 33ul 0ul (magic())) == 35)
+(* FIXME: *)
+let x509_extValue_riot_t = OCTET_STRING
+                           `inbound_envelop_tag_with_value_of`
+                           serialize_compositeDeviceID_sequence_TLV
 
-unfold
-let riot_extension_t
-= x509_extension_t OID_RIOT serialize_compositeDeviceID_sequence_TLV
+type riot_extension_t
+= { x509_extID_riot      : x:datatype_of_asn1_type OID {x == OID_RIOT};
+    x509_extCritical_riot: datatype_of_asn1_type BOOLEAN;
+    x509_extValue_riot   : x509_extValue_riot_t }
 
-// #set-options "--z3rlimit 32 --fuel 8 --ifuel 8"
-// let _ = assert (length_of_oid OID_EC_GRP_SECP256R1 == 6)
-// let _ = assert_norm (length_of_asn1_primitive_TLV (Mkbit_string_t 33ul 0ul (magic())) == 35)
+let synth_riot_extension_t
+  (x': x509_extension_t' OID_RIOT serialize_compositeDeviceID_sequence_TLV)
+: GTot (riot_extension_t)
+= { x509_extID_riot       = fst (fst x');
+    x509_extCritical_riot = snd (fst x');
+    x509_extValue_riot    = snd x' }
+
+let synth_riot_extension_t_inverse
+  (x: riot_extension_t)
+: Tot (x': x509_extension_t' OID_RIOT serialize_compositeDeviceID_sequence_TLV
+           { x == synth_riot_extension_t x' })
+= ((x.x509_extID_riot,
+    x.x509_extCritical_riot),
+    x.x509_extValue_riot)
 
 unfold
 let parse_riot_extension
 : parser parse_x509_extension_kind riot_extension_t
-= parse_x509_extension OID_RIOT serialize_compositeDeviceID_sequence_TLV
+= parse_x509_extension
+    OID_RIOT
+    serialize_compositeDeviceID_sequence_TLV
+    synth_riot_extension_t
+    ()
 
 unfold
 let serialize_riot_extension
 : serializer parse_riot_extension
-= serialize_x509_extension OID_RIOT serialize_compositeDeviceID_sequence_TLV
+= serialize_x509_extension
+    OID_RIOT
+    serialize_compositeDeviceID_sequence_TLV
+    synth_riot_extension_t
+    synth_riot_extension_t_inverse
+    ()
 
 let lemma_serialize_riot_extension_unfold
-= lemma_serialize_x509_extension_unfold OID_RIOT serialize_compositeDeviceID_sequence_TLV
+= lemma_serialize_x509_extension_unfold
+    OID_RIOT
+    serialize_compositeDeviceID_sequence_TLV
+    synth_riot_extension_t
+    synth_riot_extension_t_inverse
+    ()
 
 let lemma_serialize_riot_extension_size
-= lemma_serialize_x509_extension_size OID_RIOT serialize_compositeDeviceID_sequence_TLV
-
+= lemma_serialize_x509_extension_size
+    OID_RIOT
+    serialize_compositeDeviceID_sequence_TLV
+    synth_riot_extension_t
+    synth_riot_extension_t_inverse
+    ()
 
 let riot_extension_t_inbound
-= x509_extension_t_inbound OID_RIOT serialize_compositeDeviceID_sequence_TLV
+= x509_extension_t_inbound
+    OID_RIOT
+    serialize_compositeDeviceID_sequence_TLV
+    synth_riot_extension_t
+    synth_riot_extension_t_inverse
+    ()
 
 let parse_riot_extension_sequence_TLV
 : parser parse_x509_extension_sequence_TLV_kind riot_extension_t_inbound
-= assert (x509_extension_t_inbound OID_RIOT serialize_compositeDeviceID_sequence_TLV == riot_extension_t_inbound);
-  riot_extension_t_inbound
+= riot_extension_t_inbound
   `coerce_parser`
-  parse_x509_extension_sequence_TLV OID_RIOT serialize_compositeDeviceID_sequence_TLV
+  parse_x509_extension_sequence_TLV
+    OID_RIOT
+    serialize_compositeDeviceID_sequence_TLV
+    synth_riot_extension_t
+    synth_riot_extension_t_inverse
+    ()
 
 let serialize_riot_extension_sequence_TLV
 : serializer parse_riot_extension_sequence_TLV
 = coerce_parser_serializer
   (* p2 *) parse_riot_extension_sequence_TLV
-  (* s1 *) (serialize_x509_extension_sequence_TLV OID_RIOT serialize_compositeDeviceID_sequence_TLV)
+  (* s1 *) (serialize_x509_extension_sequence_TLV
+              OID_RIOT
+              serialize_compositeDeviceID_sequence_TLV
+              synth_riot_extension_t
+              synth_riot_extension_t_inverse
+              ())
   (* prf*) ()
 
 let lemma_serialize_riot_extension_sequence_TLV_unfold
-= lemma_serialize_x509_extension_sequence_TLV_unfold OID_RIOT serialize_compositeDeviceID_sequence_TLV
+= lemma_serialize_x509_extension_sequence_TLV_unfold
+    OID_RIOT
+    serialize_compositeDeviceID_sequence_TLV
+    synth_riot_extension_t
+    synth_riot_extension_t_inverse
+    ()
 
 let lemma_serialize_riot_extension_sequence_TLV_size
-= lemma_serialize_x509_extension_sequence_TLV_size OID_RIOT serialize_compositeDeviceID_sequence_TLV
+= lemma_serialize_x509_extension_sequence_TLV_size
+    OID_RIOT
+    serialize_compositeDeviceID_sequence_TLV
+    synth_riot_extension_t
+    synth_riot_extension_t_inverse
+    ()
 
-#push-options "--z3rlimit 64 --fuel 4 --ifuel 4"
+#push-options "--query_stats --z3rlimit 128 --fuel 4 --ifuel 4"
 let lemma_serialize_riot_extension_size_exact
   (x: riot_extension_t_inbound)
 : Lemma (
   length_of_opaque_serialization serialize_riot_extension x ==
-  length_of_asn1_primitive_TLV x.x509_extValue.riot_version + 109 /\
+  length_of_asn1_primitive_TLV x.x509_extValue_riot.riot_version + 109 /\
   length_of_opaque_serialization serialize_riot_extension x <= 115
 )
 = lemma_serialize_riot_extension_size x;
-  assert (length_of_asn1_primitive_TLV x.x509_extID == 11);
-  lemma_serialize_compositeDeviceID_sequence_TLV_size_exact x.x509_extValue;
-  assert (length_of_TLV OCTET_STRING (length_of_opaque_serialization serialize_compositeDeviceID_sequence_TLV x.x509_extValue)
-          == length_of_asn1_primitive_TLV x.x509_extValue.riot_version + 95)
+  assert (length_of_asn1_primitive_TLV x.x509_extID_riot == 11);
+  lemma_serialize_compositeDeviceID_sequence_TLV_size_exact x.x509_extValue_riot;
+  assert (length_of_TLV OCTET_STRING (length_of_opaque_serialization serialize_compositeDeviceID_sequence_TLV x.x509_extValue_riot)
+          == length_of_asn1_primitive_TLV x.x509_extValue_riot.riot_version + 95)
 
 let lemma_serialize_riot_extension_sequence_TLV_size_exact
   (x: riot_extension_t_inbound)
 : Lemma (
   length_of_opaque_serialization serialize_riot_extension_sequence_TLV x ==
-  length_of_asn1_primitive_TLV x.x509_extValue.riot_version + 111 /\
+  length_of_asn1_primitive_TLV x.x509_extValue_riot.riot_version + 111 /\
   length_of_opaque_serialization serialize_riot_extension x <= 117
 )
 = lemma_serialize_riot_extension_sequence_TLV_size x;
@@ -90,7 +145,11 @@ let serialize32_riot_extension_backwards
   (* s2 *) (serialize_riot_extension)
   (* s32*) (serialize32_x509_extension_backwards
               OID_RIOT
-              serialize32_compositeDeviceID_sequence_TLV_backwards)
+              serialize32_compositeDeviceID_sequence_TLV_backwards
+              synth_riot_extension_t
+              synth_riot_extension_t_inverse
+              synth_riot_extension_t_inverse
+              ())
   (* prf*) ()
 
 let serialize32_riot_extension_sequence_TLV_backwards
@@ -98,13 +157,12 @@ let serialize32_riot_extension_sequence_TLV_backwards
   (* s2 *) (serialize_riot_extension_sequence_TLV)
   (* s32*) (serialize32_x509_extension_sequence_TLV_backwards
               OID_RIOT
-              serialize32_compositeDeviceID_sequence_TLV_backwards)
+              serialize32_compositeDeviceID_sequence_TLV_backwards
+              synth_riot_extension_t
+              synth_riot_extension_t_inverse
+              synth_riot_extension_t_inverse
+              ())
   (* prf*) ()
-
-
-// #set-options "--z3rlimit 8"
-// let _ = assert (length_of_oid OID_EC_GRP_SECP256R1 == 6)
-// let _ = assert (length_of_asn1_primitive_TLV (Mkbit_string_t 33ul 0ul (magic())) == 35)
 
 (* helpers *)
 module B32 = FStar.Bytes
@@ -121,14 +179,14 @@ let x509_get_riot_extension
   (* Prf *) lemma_serialize_compositeDeviceID_sequence_TLV_size_exact compositeDeviceID;
 
   let riot_extension: riot_extension_t = {
-    x509_extID       = OID_RIOT;
-    x509_extCritical = false;
-    x509_extValue    = compositeDeviceID
+    x509_extID_riot       = OID_RIOT;
+    x509_extCritical_riot = false;
+    x509_extValue_riot    = compositeDeviceID
   } in
   (* Prf *) lemma_serialize_riot_extension_unfold riot_extension;
   (* Prf *) lemma_serialize_riot_extension_size   riot_extension;
-  (* Prf *) (**) lemma_serialize_asn1_oid_TLV_size riot_extension.x509_extID;
-  (* Prf *) (**) lemma_serialize_asn1_boolean_TLV_size riot_extension.x509_extCritical;
+  (* Prf *) (**) lemma_serialize_asn1_oid_TLV_size riot_extension.x509_extID_riot;
+  (* Prf *) (**) lemma_serialize_asn1_boolean_TLV_size riot_extension.x509_extCritical_riot;
 
 (*return*) riot_extension
 #pop-options
